Tests/DTLC/TrmSpec.lean
@@ -9,11 +9,6 @@ open Lp2lc.Active.DTLC
 open Lp2lc.Active.DTLC.AST
 open Lp2lc.Active.DTLC.Runtime
 
-def soundnessCounterexample {I : Index} : Trm I :=
-  .apply
-    (.apply idFn false)
-    true
-
 section eraseType
 
 example {I : Index} :
@@ -87,7 +82,7 @@ example {I : Index} [Compiletime.Env I] :
       .some ((idFnOnFalse2 : Trm I).typeEraseRecursively) := rfl
 
 example {I : Index} [Compiletime.Env I] :
-    ((soundnessCounterexample : Trm I).compile 4) =
+    ((malformedApply1 : Trm I).compile 4) =
       .some
         (.apply
           (.apply
@@ -198,7 +193,7 @@ unsafe example : ((Trm.idFnOnFalse2 : Trm RuntimeRef).eval 3) =
     .some ((Val.primitive "false") : Val RuntimeRef) := by
   rfl
 
-unsafe example : ((Trm.soundnessCounterexample : Trm RuntimeRef).eval 4) = .error := by
+unsafe example : ((Trm.malformedApply1 : Trm RuntimeRef).eval 4) = .error := by
   rfl
 
 unsafe example : ((Trm.malformedPrimitiveApply : Trm RuntimeRef).eval 0) = .outOfFuel := by
